fix alg rules, don't know how to prove yet

proof/iu_system/uni/algo_worklist/def_extra.v
@@ -25,6 +25,14 @@ Fixpoint awl_app (Γ1 Γ2 : aworklist) :=
   | aworklist_conswork Γ1' w => aworklist_conswork (awl_app Γ1' Γ2) w
   end.
 
+Fixpoint awl_rev_app (Γ1 Γ2 : aworklist) :=
+    match Γ1 with 
+    | aworklist_empty => Γ2 
+    | aworklist_constvar Γ1' X b => awl_rev_app Γ1' (aworklist_constvar Γ2 X b)
+    | aworklist_consvar Γ1' x b => awl_rev_app Γ1' (aworklist_consvar Γ2 x b)
+    | aworklist_conswork Γ1' w => awl_rev_app Γ1' (aworklist_conswork Γ2 w)
+    end.
+
 Fixpoint aenv_to_awl (E : list (atom*abind)) :=
   match E with 
   | nil => aworklist_empty
@@ -69,41 +77,41 @@ Inductive a_add_contraint_sub_etvars :
 
 
 Inductive a_update_bound
-  : aworklist ->  list (atom*abind) -> typvar -> typ -> amode_update_bound -> aworklist -> aworklist -> Prop :=
+  : aworklist -> typvar -> typ -> amode_update_bound ->  list (atom*abind) -> aworklist -> aworklist -> typ -> typ -> Prop :=
   | a_ub__lb_stop : forall Γ1 E X A LB UB Γ3, 
     X `notin` ftvar_in_typ A -> 
     a_update_bound
-     (aworklist_constvar Γ1 X (abind_bound LB UB)) E X A a_mode_ub__lower (aworklist_constvar (awl_app (aenv_to_awl E) Γ1) X (abind_bound (update_lower_bound A LB) UB)) Γ3
+     (aworklist_constvar Γ1 X (abind_bound LB UB)) X A a_mode_ub__lower E Γ1 Γ3 (update_lower_bound A LB) UB
   | a_ub__ub_stop : forall Γ1 E X A LB UB Γ3, 
     X `notin` ftvar_in_typ A -> 
     a_update_bound
-     (aworklist_constvar Γ1 X (abind_bound LB UB)) E X A a_mode_ub__upper (aworklist_constvar (awl_app (aenv_to_awl E) Γ1) X (abind_bound LB (update_upper_bound A UB))) Γ3
+     (aworklist_constvar Γ1 X (abind_bound LB UB)) X A a_mode_ub__upper E Γ1 Γ3 LB (update_upper_bound A UB)
   | a_ub__bb_stop : forall Γ1 E X A LB UB Γ3, 
     X `notin` ftvar_in_typ A -> 
     a_update_bound
-     (aworklist_constvar Γ1 X (abind_bound LB UB)) E X A a_mode_ub__both (aworklist_constvar (awl_app (aenv_to_awl E) Γ1) X (abind_bound (update_lower_bound A LB) (update_upper_bound A UB))) Γ3
-  | a_ub__etvar_move : forall Γ1 X1 LB1 UB1 E X A m Γ2 Γ3,
+     (aworklist_constvar Γ1 X (abind_bound LB UB)) X A a_mode_ub__both E Γ1 Γ3 (update_lower_bound A LB) (update_upper_bound A UB)
+  | a_ub__etvar_move : forall Γ1 X1 LB1 UB1 E X A m Γ2 Γ3 LB UB,
     X `notin` ftvar_in_abind (abind_bound LB1 UB1) ->
-    a_update_bound Γ1 E X A m Γ2 Γ3 ->
-    a_update_bound (aworklist_constvar Γ1 X1 (abind_bound LB1 UB1)) ( (X1 , (abind_bound LB1 UB1)) :: E ) X A m Γ2 Γ3
-  | a_ub__etvar_stay : forall Γ1 X1 LB1 UB1 E X A m Γ2 Γ3,
+    a_update_bound Γ1 X A m E Γ2 Γ3 LB UB ->
+    a_update_bound (aworklist_constvar Γ1 X1 (abind_bound LB1 UB1)) X A m ( (X1 , (abind_bound LB1 UB1)) :: E ) Γ2 Γ3 LB UB
+  | a_ub__etvar_stay : forall Γ1 X1 LB1 UB1 E X A m Γ2 Γ3 LB UB ,
     X1 `notin` ftvar_in_typ A /\ X1 `notin` ftvar_in_aenv E ->
-    a_update_bound Γ1 E X A m Γ2 Γ3 ->
-    a_update_bound (aworklist_constvar Γ1 X1 (abind_bound LB1 UB1)) E X A m Γ2 (aworklist_constvar Γ3 X1 (abind_bound LB1 UB1))
-  | a_ub__tvar_stay : forall Γ1 X1 E X A m Γ2 Γ3,
+    a_update_bound Γ1 X A m E Γ2 Γ3 LB UB ->
+    a_update_bound (aworklist_constvar Γ1 X1 (abind_bound LB1 UB1)) X A m E Γ2 (aworklist_constvar Γ3 X1 (abind_bound LB1 UB1)) LB UB
+  | a_ub__tvar_stay : forall Γ1 X1 E X A m Γ2 Γ3 LB UB ,
     X1 `notin` ftvar_in_typ A /\ X1 `notin` ftvar_in_aenv E ->
-    a_update_bound Γ1 E X A m Γ2 Γ3 ->
-    a_update_bound (aworklist_constvar Γ1 X1 abind_tvar_empty) E X A m Γ2 (aworklist_constvar Γ3 X1 abind_tvar_empty)
-  | a_ub__stvar_stay : forall Γ1 X1 E X A m Γ2 Γ3,
+    a_update_bound Γ1 X A m E Γ2 Γ3 LB UB  ->
+    a_update_bound (aworklist_constvar Γ1 X1 abind_tvar_empty) X A m E Γ2 (aworklist_constvar Γ3 X1 abind_tvar_empty) LB UB  
+  | a_ub__stvar_stay : forall Γ1 X1 E X A m Γ2 Γ3 LB UB ,
     X1 `notin` ftvar_in_typ A /\ X1 `notin` ftvar_in_aenv E ->
-    a_update_bound Γ1 E X A m Γ2 Γ3 ->
-    a_update_bound (aworklist_constvar Γ1 X1 abind_stvar_empty) E X A m Γ2 (aworklist_constvar Γ3 X1 abind_stvar_empty)
-  | a_ub__w_stay : forall Γ1 w1 E X A m Γ2 Γ3,
-    a_update_bound Γ1 E X A m Γ2 Γ3 ->
-    a_update_bound (aworklist_conswork Γ1 w1) E X A m Γ2 (aworklist_conswork Γ3 w1)
-  | a_ub__var_stay : forall Γ1 x1 b1 E X A m Γ2 Γ3,
-    a_update_bound Γ1 E X A m Γ2 Γ3 ->
-    a_update_bound (aworklist_consvar Γ1 x1 b1) E X A m Γ2 (aworklist_consvar Γ3 x1 b1) 
+    a_update_bound Γ1 X A m E Γ2 Γ3 LB UB ->
+    a_update_bound (aworklist_constvar Γ1 X1 abind_stvar_empty) X A m E Γ2  (aworklist_constvar Γ3 X1 abind_stvar_empty) LB UB
+  | a_ub__w_stay : forall Γ1 w1 E X A m Γ2 Γ3 LB UB,
+    a_update_bound Γ1 X A m E Γ2 Γ3 LB UB ->
+    a_update_bound (aworklist_conswork Γ1 w1) X A m E Γ2 (aworklist_conswork Γ3 w1) LB UB 
+  | a_ub__var_stay : forall Γ1 x1 b1 E X A m Γ2 Γ3 LB UB,
+    a_update_bound Γ1 X A m E Γ2 Γ3 LB UB  ->
+    a_update_bound (aworklist_consvar Γ1 x1 b1) X A m E Γ2 (aworklist_consvar Γ3 x1 b1) LB UB 
   .
 
 (* defns Jaworklist_reduction *)
@@ -148,42 +156,42 @@ Inductive a_wl_red : aworklist -> Prop :=    (* defn a_wl_red *)
  | d_wl_del__sub_arrow1 : forall (L:vars) (Γ:aworklist) (X:typvar) (A1 A2 B1 B2:typ),
       binds ( X )  ( (abind_bound B1 B2) ) (  ( awl_to_aenv  Γ  )  )  ->
       ( a_smono_typ   ( awl_to_aenv  Γ  )     ( (typ_arrow A1 A2) )   -> False )  ->
-      (forall X1, X1 `notin` L -> forall X2, X2 `notin` (L `union` singleton X1) -> forall Γ2 Γ3,
-        (a_update_bound  (aworklist_constvar (aworklist_constvar Γ X1 (abind_bound typ_bot typ_top)) X2 (abind_bound typ_bot typ_top))   nil   X   (typ_arrow (typ_var_f X1) (typ_var_f X2))  a_mode_ub__upper  Γ2   Γ3 ) ->
-        (a_wl_red (aworklist_conswork  (   ( awl_app  Γ3   Γ2  )   )  (work_sub (typ_arrow (typ_var_f X1) (typ_var_f X2)) (typ_arrow A1 A2)))) ) ->
+      (forall X1, X1 `notin` L -> forall X2, X2 `notin` (L `union` singleton X1) -> forall Γ2 Γ3 E LB UB,
+        (a_update_bound  (aworklist_constvar (aworklist_constvar Γ X1 (abind_bound typ_bot typ_top)) X2 (abind_bound typ_bot typ_top))   X   (typ_arrow (typ_var_f X1) (typ_var_f X2))  a_mode_ub__upper E Γ2 Γ3 LB UB ) ->
+        (a_wl_red (aworklist_conswork  (   (awl_rev_app Γ3 (aworklist_constvar (awl_rev_app (aenv_to_awl E) Γ2) X (abind_bound LB UB)) )   )  (work_sub (typ_arrow (typ_var_f X1) (typ_var_f X2)) (typ_arrow A1 A2)))) ) ->
      a_wl_red (aworklist_conswork Γ (work_sub (typ_var_f X) (typ_arrow A1 A2)))
  | d_wl_del__sub_arrow2 : forall (L:vars) (Γ:aworklist) (A1 A2:typ) (X:typvar) (B1 B2:typ),
       binds ( X )  ( (abind_bound B1 B2) ) (  ( awl_to_aenv  Γ  )  )  ->
       ( a_smono_typ   ( awl_to_aenv  Γ  )     ( (typ_arrow A1 A2) )   -> False )  ->
-      (forall X1, X1 `notin` L -> forall X2, X2 `notin` (L `union` singleton X1) -> forall Γ2 Γ3,
-             (a_update_bound  (aworklist_constvar (aworklist_constvar Γ X1 (abind_bound typ_bot typ_top)) X2 (abind_bound typ_bot typ_top))   nil   X   (typ_arrow (typ_var_f X1) (typ_var_f X2))  a_mode_ub__lower  Γ2   Γ3 ) ->
-            a_wl_red (aworklist_conswork  (  ( awl_app  Γ3   Γ2  )    )  (work_sub (typ_arrow A1 A2) (typ_arrow (typ_var_f X1) (typ_var_f X2)))) )->
+      (forall X1, X1 `notin` L -> forall X2, X2 `notin` (L `union` singleton X1) -> forall Γ2 Γ3 E LB UB,
+             (a_update_bound  (aworklist_constvar (aworklist_constvar Γ X1 (abind_bound typ_bot typ_top)) X2 (abind_bound typ_bot typ_top))   X   (typ_arrow (typ_var_f X1) (typ_var_f X2))  a_mode_ub__lower  E Γ2  Γ3 LB UB ) ->
+            a_wl_red (aworklist_conswork  (  (awl_rev_app Γ3 (aworklist_constvar (awl_rev_app (aenv_to_awl E) Γ2) X (abind_bound LB UB)) )   )  (work_sub (typ_arrow A1 A2) (typ_arrow (typ_var_f X1) (typ_var_f X2)))) )->
      a_wl_red (aworklist_conswork Γ (work_sub (typ_arrow A1 A2) (typ_var_f X)))
- | d_wl_del__sub_etvar1 : forall (L:vars) (Γ Γ2 Γ3:aworklist) (Y X:typvar) (B1 B2 B3 B4:typ),
+ | d_wl_del__sub_etvar1 : forall (L:vars) (E:aenv) (Γ Γ2 Γ3:aworklist) (Y X:typvar) (B1 B2 B3 B4 LB UB:typ),
       binds ( X )  ( (abind_bound B1 B2) ) (  ( awl_to_aenv  Γ  )  )  ->
       binds ( Y )  ( (abind_bound B3 B4) ) (  ( awl_to_aenv  Γ  )  )  ->     a_evs_in_wl Γ X Y ->
       a_evs_in_wl Γ X Y ->
-      (a_update_bound  Γ   nil   X   (typ_var_f Y)  a_mode_ub__lower  Γ2   Γ3 )  ->
-       a_wl_red  (   ( awl_app  Γ3   Γ2  )   )  ->
+      (a_update_bound  Γ  X   (typ_var_f Y)  a_mode_ub__lower  E Γ2   Γ3 LB UB)  ->
+       a_wl_red  (   (awl_rev_app Γ3 (aworklist_constvar (awl_rev_app (aenv_to_awl E) Γ2) X (abind_bound LB UB)) )  )  ->
      a_wl_red (aworklist_conswork Γ (work_sub (typ_var_f Y) (typ_var_f X)))
- | d_wl_del__sub_etvar2 : forall (L:vars) (Γ Γ2 Γ3:aworklist) (X Y:typvar) (B1 B2 B3 B4:typ),
+ | d_wl_del__sub_etvar2 : forall (L:vars) (E:aenv) (Γ Γ2 Γ3:aworklist) (X Y:typvar) (B1 B2 B3 B4 LB UB:typ),
       binds ( X )  ( (abind_bound B1 B2) ) (  ( awl_to_aenv  Γ  )  )  ->
       binds ( Y )  ( (abind_bound B3 B4) ) (  ( awl_to_aenv  Γ  )  )  ->
       a_evs_in_wl Γ X Y ->
-      (a_update_bound  Γ   nil   X   (typ_var_f Y)  a_mode_ub__upper  Γ2   Γ3 )  ->
-      a_wl_red  (   ( awl_app  Γ3   Γ2  )   )  ->
+      (a_update_bound  Γ  X   (typ_var_f Y)  a_mode_ub__upper E Γ2   Γ3 LB UB)  ->
+      a_wl_red  (   (awl_rev_app Γ3 (aworklist_constvar (awl_rev_app (aenv_to_awl E) Γ2) X (abind_bound LB UB)) )  )  ->
      a_wl_red (aworklist_conswork Γ (work_sub (typ_var_f X) (typ_var_f Y)))
- | d_wl_del__sub_etvarmono1 : forall (L:vars) (Γ Γ2 Γ3:aworklist) (A1:typ) (X:typvar) (B1 B2:typ),
+ | d_wl_del__sub_etvarmono1 : forall (L:vars)  (E:aenv) (Γ Γ2 Γ3:aworklist) (A1:typ) (X:typvar) (B1 B2 LB UB:typ),
       binds ( X )  ( (abind_bound B1 B2) ) (  ( awl_to_aenv  Γ  )  )  ->
      a_smono_typ  ( awl_to_aenv  Γ  )  A1 ->
-     (a_update_bound  Γ   nil   X   A1  a_mode_ub__lower  Γ2   Γ3 )  ->
-      a_wl_red  (   ( awl_app  Γ3   Γ2  )   ) ->
+     (a_update_bound  Γ  X   A1  a_mode_ub__lower E Γ2 Γ3 LB UB )  ->
+      a_wl_red  (   (awl_rev_app Γ3 (aworklist_constvar (awl_rev_app (aenv_to_awl E) Γ2) X (abind_bound LB UB)) ) ) ->
      a_wl_red (aworklist_conswork Γ (work_sub A1 (typ_var_f X)))
- | d_wl_del__sub_etvarmono2 : forall (L:vars) (Γ Γ2 Γ3:aworklist) (X:typvar) (B1 A1 A2:typ),
+ | d_wl_del__sub_etvarmono2 : forall (L:vars) (E:aenv) (Γ Γ2 Γ3:aworklist) (X:typvar) (B1 A1 A2 LB UB:typ),
       binds ( X )  ( (abind_bound A1 A2) ) (  ( awl_to_aenv  Γ  )  )  ->
      a_smono_typ  ( awl_to_aenv  Γ  )  B1 ->
-     a_update_bound  Γ   nil   X   B1  a_mode_ub__upper  Γ2   Γ3 ->
-      a_wl_red  (   ( awl_app  Γ3   Γ2  )   ) ->
+     a_update_bound  Γ  X   B1  a_mode_ub__upper E  Γ2   Γ3 LB UB->
+      a_wl_red  (   (awl_rev_app Γ3 (aworklist_constvar (awl_rev_app (aenv_to_awl E) Γ2) X (abind_bound LB UB)) )  ) ->
      a_wl_red (aworklist_conswork Γ (work_sub (typ_var_f X) B1))
  | d_wl_del__sub_intersection1 : forall (Γ:aworklist) (A1 B1 B2:typ),
      a_wl_red (aworklist_conswork (aworklist_conswork Γ (work_sub A1 B1)) (work_sub A1 B2)) ->
@@ -211,9 +219,9 @@ Inductive a_wl_red : aworklist -> Prop :=    (* defn a_wl_red *)
      a_wl_red (aworklist_conswork Γ (work_check (exp_abs e) (typ_arrow A1 A2)))
  | d_wl_del__chk_absevar : forall (L:vars) (Γ:aworklist) (e:exp) (X:typvar) (A1 A2:typ) (X1 X2:typvar),
       binds ( X )  ( (abind_bound A1 A2) ) (  ( awl_to_aenv  Γ  )  )  ->
-      (  forall x X1 X2 Γ2 Γ3, x `notin` L -> X1 `notin` (L `union` (singleton x)) -> X2 `notin` (L `union` singleton x `union` singleton X1) -> 
-            (a_update_bound  (aworklist_constvar (aworklist_constvar Γ X1 (abind_bound typ_bot typ_top)) X2 (abind_bound typ_bot typ_top))  nil   X   (typ_arrow (typ_var_f X1) (typ_var_f X2))  a_mode_ub__both  Γ2   Γ3 )  ->
-            a_wl_red (aworklist_conswork (aworklist_consvar  (   ( awl_app  Γ3   Γ2  )   )  x (abind_typ (typ_var_f X1))) (work_check  ( open_exp_wrt_exp e (exp_var_f x) )  (typ_var_f X2))) ) ->
+      (  forall x, x `notin` L -> forall X1, X1 `notin` (L `union` (singleton x)) -> forall X2, X2 `notin` (L `union` singleton x `union` singleton X1) -> forall Γ2 Γ3 E LB UB,
+            (a_update_bound  (aworklist_constvar (aworklist_constvar Γ X1 (abind_bound typ_bot typ_top)) X2 (abind_bound typ_bot typ_top))  X   (typ_arrow (typ_var_f X1) (typ_var_f X2))  a_mode_ub__both E  Γ2   Γ3 LB UB)  ->
+            a_wl_red (aworklist_conswork (aworklist_consvar  (   (awl_rev_app Γ3 (aworklist_constvar (awl_rev_app (aenv_to_awl E) Γ2) X (abind_bound LB UB)) )  )  x (abind_typ (typ_var_f X1))) (work_check  ( open_exp_wrt_exp e (exp_var_f x) )  (typ_var_f X2))) ) ->
      a_wl_red (aworklist_conswork Γ (work_check (exp_abs e) (typ_var_f X)))
  | d_wl_del__chk_abstop : forall (L:vars) (Γ:aworklist) (e:exp),
       ( forall x , x \notin  L  -> a_wl_red (aworklist_conswork (aworklist_consvar Γ x (abind_typ typ_bot)) (work_check  ( open_exp_wrt_exp e (exp_var_f x) )  typ_top)) )  ->
@@ -274,9 +282,9 @@ Inductive a_wl_red : aworklist -> Prop :=    (* defn a_wl_red *)
      a_wl_red (aworklist_conswork Γ (work_unioninfabs (typ_arrow B2 C2) (typ_arrow B1 C1) c))
  | d_wl_del__infabs_evar : forall (L:vars) (Γ:aworklist) (X:typvar) (c:cont) (A1 A2:typ) (X1 X2:typvar),
      binds ( X )  ( (abind_bound A1 A2) ) (  ( awl_to_aenv  Γ  )  )  ->
-     (forall X1, X1 `notin` L -> forall X2, X2 `notin` (L `union` singleton X1) -> forall Γ2 Γ3,
-         (a_update_bound  (aworklist_constvar (aworklist_constvar Γ X1 (abind_bound typ_bot typ_top)) X2 (abind_bound typ_bot typ_top))   nil   X   (typ_arrow (typ_var_f X1) (typ_var_f X2))  a_mode_ub__both  Γ2   Γ3 )  /\
-       a_wl_red (aworklist_conswork  (   ( awl_app  Γ3   Γ2  )   )  (work_infabs (typ_arrow (typ_var_f X1) (typ_var_f X2)) c))
+     (forall X1, X1 `notin` L -> forall X2, X2 `notin` (L `union` singleton X1) -> forall E Γ2 Γ3 LB UB,
+         (a_update_bound  (aworklist_constvar (aworklist_constvar Γ X1 (abind_bound typ_bot typ_top)) X2 (abind_bound typ_bot typ_top))  X   (typ_arrow (typ_var_f X1) (typ_var_f X2))  a_mode_ub__both  E  Γ2   Γ3 LB UB)  /\
+       a_wl_red (aworklist_conswork  (   (awl_rev_app Γ3 (aworklist_constvar (awl_rev_app (aenv_to_awl E) Γ2) X (abind_bound LB UB)) )   )  (work_infabs (typ_arrow (typ_var_f X1) (typ_var_f X2)) c))
      ) ->
     a_wl_red (aworklist_conswork Γ (work_infabs (typ_var_f X) c))
  | d_wl_del__inf_tapp : forall (Γ:aworklist) (e:exp) (B:typ) (c:cont),
